queryimpl verifies in 35s

Impl/QueryModel.i.dfy
@@ -33,63 +33,53 @@ module QueryModel {
 
   // == query ==
 
-  predicate queryInv(s: BBC.Variables, key: Key, msg: Message, ref: BT.G.Reference, 
-    io: IO, counter: uint64, lookup: seq<BT.Layer>)
+  predicate queryInv(s: BBC.Variables, querykey: Key, key: Key, msg: Message, ref: BT.G.Reference, 
+    io: IO, counter: int , lookup: seq<BT.Layer>)
   {
     && s.Ready?
     && BBC.Inv(s)
     && io.IOInit?
     && ref in s.ephemeralIndirectionTable.graph
     && counter >= 0
-    && (|lookup| == 0 ==> ref == BT.G.Root())
-    && (msg.Define? ==> |lookup| > 0)
-    && (|lookup| > 0 ==> BT.WFLookupForKey(lookup, lookup[0].currentKey))
-    && (!msg.Define? ==> |lookup| > 0 ==> Last(lookup).readOp.node.children.Some?)
-    && (!msg.Define? ==> |lookup| > 0 ==> Last(lookup).readOp.node.children.value[
-          Route(Last(lookup).readOp.node.pivotTable, Last(lookup).currentKey)] == ref)
-    && (!msg.Define? ==> |lookup| > 0 ==> TranslateKey(Last(lookup).readOp.node.pivotTable, 
-          Last(lookup).readOp.node.edgeTable, Last(lookup).currentKey) == key)
-    && (forall i | 0 <= i < |lookup| :: BT.WFNode(lookup[i].readOp.node))
+    && (|lookup| == 0 ==> ref == BT.G.Root() && querykey == key)
+    && (msg.Define? ==> |lookup| > 0 && BT.WFLookupForKey(lookup, querykey))
+    && (!msg.Define? ==> |lookup| > 0 ==>
+        && BT.WFLookupForKey(lookup, querykey)
+        && Last(lookup).readOp.node.children.Some?
+        && Last(lookup).readOp.node.children.value[Route(Last(lookup).readOp.node.pivotTable, Last(lookup).currentKey)] == ref
+        && TranslateKey(Last(lookup).readOp.node.pivotTable, Last(lookup).readOp.node.edgeTable, Last(lookup).currentKey) == key)
     && (forall i | 0 <= i < |lookup| :: lookup[i].readOp.ref in s.ephemeralIndirectionTable.graph)
     && (forall i | 0 <= i < |lookup| :: MapsTo(s.cache, lookup[i].readOp.ref, lookup[i].readOp.node))
-    && (forall i | 0 <= i < |lookup| :: BoundedKey(lookup[i].readOp.node.pivotTable, lookup[i].currentKey))
     && (ref in s.ephemeralIndirectionTable.graph)
     && (BT.LookupVisitsWellMarshalledBuckets(lookup) ==> msg == BT.InterpretLookup(lookup))
   }
 
-  function {:opaque} new_lookup(lookup: seq<BT.Layer>, ref: BT.G.Reference, node: BT.G.Node, key: Key) : seq<BT.Layer>
+  function new_lookup(lookup: seq<BT.Layer>, ref: BT.G.Reference, node: BT.G.Node, key: Key) : seq<BT.Layer>
   {
     lookup + [BT.Layer(BT.G.ReadOp(ref, node), key)]
   }
 
-  lemma AugmentLookup(lookup': seq<BT.Layer>, lookup: seq<BT.Layer>, ref: BT.G.Reference, node: BT.G.Node, 
+  lemma AugmentLookup(lookup': seq<BT.Layer>, lookup: seq<BT.Layer>, querykey: Key, ref: BT.G.Reference, node: BT.G.Node, 
     key: Key, cache: map<BT.G.Reference, BT.G.Node>, graph: map<BT.G.Reference, seq<BT.G.Reference>>)
   requires lookup' == new_lookup(lookup, ref, node, key)
-  requires |lookup| > 0 ==> BT.WFLookupForKey(lookup, lookup[0].currentKey)
-  requires forall i | 0 <= i < |lookup| :: BT.WFNode(lookup[i].readOp.node)
+  requires |lookup| == 0 ==> ref == BT.G.Root() && querykey == key
+  requires |lookup| > 0 ==>
+    && BT.WFLookupForKey(lookup, querykey)
+    && Last(lookup).readOp.node.children.Some?
+    && Last(lookup).readOp.node.children.value[Route(Last(lookup).readOp.node.pivotTable, Last(lookup).currentKey)] == ref
+    && TranslateKey(Last(lookup).readOp.node.pivotTable, Last(lookup).readOp.node.edgeTable, Last(lookup).currentKey) == key
   requires forall i | 0 <= i < |lookup| :: lookup[i].readOp.ref in graph
   requires forall i | 0 <= i < |lookup| :: MapsTo(cache, lookup[i].readOp.ref, lookup[i].readOp.node)
-  requires forall i | 0 <= i < |lookup| :: BoundedKey(lookup[i].readOp.node.pivotTable, lookup[i].currentKey)
-  requires |lookup| == 0 ==> ref == BT.G.Root()
-  requires |lookup| > 0 ==> Last(lookup).readOp.node.children.Some?
-  requires |lookup| > 0 ==> Last(lookup).readOp.node.children.value[
-        Route(Last(lookup).readOp.node.pivotTable, Last(lookup).currentKey)] == ref
-  requires |lookup| > 0 ==> TranslateKey(Last(lookup).readOp.node.pivotTable, 
-        Last(lookup).readOp.node.edgeTable, Last(lookup).currentKey) == key
   requires BT.WFNode(node)
   requires MapsTo(cache, ref, node);
   requires BoundedKey(node.pivotTable, key)
   requires ref in graph
-  ensures |lookup'| > 0 && BT.WFLookupForKey(lookup', lookup'[0].currentKey)
+  ensures |lookup'| > 0 && BT.WFLookupForKey(lookup', querykey)
   ensures Last(lookup').readOp.node == node
   ensures BT.InterpretLookup(lookup') == Messages.Merge(BT.InterpretLookup(lookup), BT.NodeLookup(node, key))
-  ensures forall i | 0 <= i < |lookup'| :: BT.WFNode(lookup'[i].readOp.node)
   ensures forall i | 0 <= i < |lookup'| :: lookup'[i].readOp.ref in graph
   ensures forall i | 0 <= i < |lookup'| :: MapsTo(cache, lookup'[i].readOp.ref, lookup'[i].readOp.node)
-  ensures forall i | 0 <= i < |lookup'| :: BoundedKey(lookup'[i].readOp.node.pivotTable, lookup'[i].currentKey)
   {
-    reveal_new_lookup();
-
     forall idx | BT.ValidLayerIndex(lookup', idx) && idx < |lookup'| - 1
     ensures BT.LookupFollowsChildRefAtLayer(lookup', idx)
     ensures BT.LookupFollowsChildEdgeAtLayer(lookup', idx)
