Impl/QueryImpl.i.dfy
@@ -38,24 +38,22 @@ module QueryImpl {
   import opened BoundedPivotsLib
   import opened TranslationLib
   import opened DiskOpModel
-
-  // import PBS = PivotBetreeSpec`Internal
   import opened InterpretationDiskOps
   import opened ViewOp
 
   // == query ==
 
-  method queryIterate(linear inout s: ImplVariables, key: Key, msg: Message,
+  method queryIterate(linear inout s: ImplVariables, querykey: Key, key: Key, msg: Message,
     ref: BT.G.Reference, io: DiskIOHandler, counter: uint64, ghost lookup: seq<BT.Layer>)
   returns (res: Option<Value>)
 
   requires old_s.Inv()
-  requires queryInv(old_s.I(), key, msg, ref, IIO(io), counter, lookup)
+  requires queryInv(old_s.I(), querykey, key, msg, ref, IIO(io), counter, lookup)
   requires !msg.Define?
   requires io.initialized()
 
   modifies io
-  decreases counter
+  decreases counter, 1
   ensures s.WFBCVars()
 
   ensures ValidDiskOp(diskOp(IIO(io)))
@@ -63,7 +61,7 @@ module QueryImpl {
   ensures res.Some? ==>
       BBC.Next(old_s.I(), s.I(),
           IDiskOp(diskOp(IIO(io))).bdop,
-          AdvanceOp(UI.GetOp(key, res.value), false));
+          AdvanceOp(UI.GetOp(querykey, res.value), false));
   ensures res.None? ==>
       IOModel.betree_next_dop(old_s.I(), s.I(),
           IDiskOp(diskOp(IIO(io))).bdop)
@@ -89,66 +87,52 @@ module QueryImpl {
           ghost var oldIVars := s.I();
           LruModel.LruUse(s.lru.Queue(), ref);
           inout s.lru.Use(ref);
-          assert oldIVars == s.I();
 
+          ghost var node := s.cache.I()[ref];
+              
           var r := Pivots.ComputeRoute(pivots, key);
           ghost var bucket := node.buckets[r];
           var kmtMsg := s.cache.GetMessage(ref, r, key);
           var newmsg := if kmtMsg.Some? then ValueMessage.Merge(msg, kmtMsg.value) else msg;
 
           ghost var newlookup := new_lookup(lookup, ref, node, key);
-          AugmentLookup(newlookup, lookup, ref, node, key, s.cache.I(), s.ephemeralIndirectionTable.graph);
+          AugmentLookup(newlookup, lookup, querykey, ref, node, key, s.cache.I(), s.ephemeralIndirectionTable.graph);
 
-          assume BT.LookupVisitsWellMarshalledBuckets(newlookup) ==> BucketWellMarshalled(bucket);
-          assume BT.LookupVisitsWellMarshalledBuckets(newlookup) ==> BT.LookupVisitsWellMarshalledBuckets(lookup);
-          // by {
-          //   reveal_new_lookup();
-          // }
+          assert BT.LookupVisitsWellMarshalledBuckets(newlookup) ==> 
+            && BucketWellMarshalled(bucket) 
+            && BT.LookupVisitsWellMarshalledBuckets(lookup);
 
-          // assert BT.LookupVisitsWellMarshalledBuckets(newlookup) ==> BucketWellMarshalled(bucket);
-          // assert BT.LookupVisitsWellMarshalledBuckets(newlookup) ==> BT.LookupVisitsWellMarshalledBuckets(lookup)
-          // by {
-          //   reveal_new_lookup();
-          // }
-
-          assert |newlookup| > 0;
-          var querykey := newlookup[0].currentKey;
-
-          // might be better to divide into smaller cases 
-          // taking a long time to verify
-
-          if (newmsg.Define?) {  
+          if (newmsg.Define?) {
             res := Some(newmsg.value);
-
             assert BT.ValidQuery(BT.LookupQuery(querykey, res.value, newlookup));
+
             assert BBC.BetreeMove(old_s.I(), s.I(),
-              IDiskOp(diskOp(IIO(io))).bdop,
-              AdvanceOp(UI.GetOp(querykey, res.value), false),
-              BT.BetreeQuery(BT.LookupQuery(querykey, res.value, newlookup)));
+                IDiskOp(diskOp(IIO(io))).bdop,
+                AdvanceOp(UI.GetOp(querykey, res.value), false),
+                BT.BetreeQuery(BT.LookupQuery(querykey, res.value, newlookup)));
+
             assert IOModel.stepsBetree(old_s.I(), s.I(),
-              AdvanceOp(UI.GetOp(querykey, res.value), false),
-              BT.BetreeQuery(BT.LookupQuery(querykey, res.value, newlookup)));
+                AdvanceOp(UI.GetOp(querykey, res.value), false),
+                BT.BetreeQuery(BT.LookupQuery(querykey, res.value, newlookup)));
           } else {
-            assume false;
+            if children.Some? {
+              BookkeepingModel.lemmaChildInGraph(s.I(), ref, children.value[r]);
+              var newkey := ComputeTranslateKey(pivots, edges, key, r);
+              res := queryIterate(inout s, querykey, newkey, newmsg, children.value[r], io, counter - 1, newlookup);
+            } else {
+              res := Some(ValueType.DefaultValue());
+              assert BC.OpTransaction(old_s.I(), s.I(),
+                BT.BetreeStepOps(BT.BetreeQuery(BT.LookupQuery(querykey, res.value, newlookup))));
 
-            // if children.Some? {
-            //   BookkeepingModel.lemmaChildInGraph(s.I(), ref, children.value[r]);
-            //   var newkey := ComputeTranslateKey(pivots, edges, key, r);
-            //   res := queryIterate(inout s, newkey, newmsg, children.value[r], io, counter - 1, newlookup);
-            // } else {
-            //   res := Some(ValueType.DefaultValue());
-            //   assert BC.OpTransaction(old_s.I(), s.I(),
-            //     BT.BetreeStepOps(BT.BetreeQuery(BT.LookupQuery(querykey, res.value, newlookup))));
+              assert BBC.BetreeMove(old_s.I(), s.I(),
+                IDiskOp(diskOp( IIO(io) )).bdop,
+                AdvanceOp(UI.GetOp(querykey, res.value), false),
+                BT.BetreeQuery(BT.LookupQuery(querykey, res.value, newlookup)));
 
-            //   assert BBC.BetreeMove(old_s.I(), s.I(),
-            //     IDiskOp(diskOp( IIO(io) )).bdop,
-            //     AdvanceOp(UI.GetOp(querykey, res.value), false),
-            //     BT.BetreeQuery(BT.LookupQuery(querykey, res.value, newlookup)));
-
-            //   assert IOModel.stepsBetree(old_s.I(), s.I(),
-            //     AdvanceOp(UI.GetOp(querykey, res.value), false),
-            //     BT.BetreeQuery(BT.LookupQuery(querykey, res.value, newlookup)));
-            // }
+              assert IOModel.stepsBetree(old_s.I(), s.I(),
+                AdvanceOp(UI.GetOp(querykey, res.value), false),
+                BT.BetreeQuery(BT.LookupQuery(querykey, res.value, newlookup)));
+            }
           }
         }
       }
@@ -177,6 +161,6 @@ module QueryImpl {
     var msg := ValueMessage.IdentityMessage();
     var counter: uint64 := 40;
 
-    res := queryIterate(inout s, key, msg, ref, io, counter, []);
+    res := queryIterate(inout s, key, key, msg, ref, io, counter, []);
   }
 }
